\chapter{Proofs}

\section{Basic proofs}

\subsection{Eq (\ref{eq:hamiltonain-exponential})}
\label{appendix-proof-1}

For convenience, $\mathbf{v} = \mathcal{H}$
\begin{equation}
    \exp(- \theta \mathbf{v} \cdot \matbf{\sigma}) = \sum_{k=0} \frac{(-i\theta \mathbf{v} \cdot \mathbf{\sigma})^k}{k!} \\
\end{equation}

Pauli-matrices have next relationship,
\begin{align}
    \sigma_j \sigma_k = \dela_{jk}  + i\sum_{l} \epsilon_{jkl}\sigma_l \\
    [\sigma_j, \sigma_k] =& (\delta_{jk} - \delta_{kj}) + i (\sum_{l} \epsilon_{jkl}\sigma_l - \sum_{m} \epsilon_{jkm}\sigma_m)\\
     =& i (\sum_{l, m} \epsilon{jkl} \delta_l + \epsilon_{jkm} \delta_m)\\
     = & \begin{cases}
        2 i \epsilon_{jkl}\delta_l & j \neq k \\
        0 & j=k
     \end{cases}
\end{align}
then,
\begin{align}
    (\mathbf{v} \cdot \mathbf{\sigma})^{2n +1} = |\mathbf{v}|^{2n+1} (\hat{\mathbf{v}} \cdot \mathbf{\sigma})
    (\mathbf{v} \cdot \mathbf{\sigma})^{2n} = |\mathbf{v}|^{2n} (\hat{I})
\end{align}.
therefore,

\begin{align}
    =& \sum_{k=0}^\infty \frac{(-i)^{2k}}{(2k)!} (\theta |\mathbf{v}|)^{2k} \hat{I} + \sum_{k=0}^\infty \frac{(-i)^{2k+1}}{(2k+1)!} (\theta |\mathbf{v}|)^{2k+1} (\hat{\mathbf{v}} \cdot \mathbf{\sigma})\\
    =& \sum_{k=0}^\infty \frac{(-1)^{k}}{(2k)!} (\theta |\mathbf{v}|)^{2k} \hat{I} -i \sum_{k=0}^\infty \frac{(-1)^{k}}{(2k+1)!} (\theta |\mathbf{v}|)^{2k+1} (\hat{\mathbf{v}} \cdot \mathbf{\sigma}) \\
    = & \cos(\theta |\mathbf{v}|) \hat{I} - i \sin(\theta |\mathbf{v}|) (\hat{\mathbf{v}} \cdot \mathbf{\sigma})
\end{align}